

$$\int_0^t K(t-\tau) \dot{v}(\tau) d\tau; \quad v(\tau) = \dot{z}(\tau)$$

$$K(s) V(s); \quad K(s) \text{ can be written as } \underline{C}_r^T (s \underline{I} - \underline{A}_r)^{-1} \underline{B}_r = \frac{b_n s^n + b_{n-1} s^{n-1} + \dots + b_1 s + b_0}{s^n + a_{n-1} s^{n-1} + \dots + a_1 s + a_0}$$

here $b_n = 0$

$$\dot{z}_r(t) = \underline{A}_r z_r(t) + \underline{B}_r \dot{v}(t)$$

$$(s \underline{I} - \underline{A}_r) \underline{Z}_r(s) = \underline{B}_r V(s)$$

$$\underline{Z}_r(s) = (s \underline{I} - \underline{A}_r)^{-1} \underline{B}_r V(s)$$

$$\underline{C}_r^T \underline{Z}_r(s) = \underbrace{\underline{C}_r^T (s \underline{I} - \underline{A}_r)^{-1} \underline{B}_r}_{K(s)} V(s)$$

$$\underline{C}_r^T \underline{Z}_r(t) = k(t) * \dot{v}(t) = \int_0^t K(t-\tau) \dot{v}(\tau) d\tau = y_r(t)$$

①: radiation force:

$$F_{rad}(t) = -m_{\infty} \ddot{z}(t) - \int_0^t K(t-\tau) \dot{v}(\tau) d\tau$$

m_{∞} : added mass at infinite frequency; $K(t)$: radiation impulse.

②: wave excitation force:

$$F_{exc}(t) = \text{Real} \left\{ \frac{H}{2} F_{exc}(\omega, \theta) e^{j\omega t} \right\}$$

H : amplitude of wave; calculate $F_{exc}(\omega, \theta)$?

③: hydrostatic restoring force:

$$F_h(t) = \rho g V_i = \rho g (V_0 - S z(t)); \quad \text{set: } V_0 = 0$$

$$\text{Let: hydrostatic stiffness } S_h = \rho g S \Rightarrow F_h(t) = -S_h z(t)$$

$$m \ddot{z}(t) = F_{rad} + F_{exc} + F_{pro} + F_h$$

$$m \ddot{z}(t) = -m_{\infty} \ddot{z}(t) - \int_0^t K(t-\tau) \dot{z}(\tau) d\tau + F_{exc}(t) + F_{pro}(t) - S_h z(t); \quad v(t) = \dot{z}(t)$$

$$(m_{\infty} + m) \ddot{z}(t) + S_h z(t) + \underbrace{\int_0^t K(t-\tau) \dot{z}(\tau) d\tau}_{\underline{C}_r^T \underline{Z}_r(t)} = F_{exc}(t) + F_{pro}(t)$$

$$(m_{\infty} + m) \ddot{z}(t) + S_h z(t) + \underline{C}_r^T \underline{Z}_r(t) = F_{exc}(t) + F_{pro}(t)$$

$$\ddot{z}(t) = -\frac{1}{m+m_{\infty}} S_h z(t) - \frac{1}{m+m_{\infty}} \underline{C}_r^T \underline{Z}_r(t) + \frac{1}{m+m_{\infty}} F_{exc}(t) + \frac{1}{m+m_{\infty}} F_{pro}(t)$$

$$\text{Let: } \underline{x}(t) = (\underline{x}_1(t) \quad \underline{x}_2(t) \quad \underline{x}_3(t))^T = (z(t) \quad \dot{z}(t) \quad \underline{Z}_r(t))^T$$